Analysis typeclass added

coq_general_theory/evolution_aware_theory_v2.v
@@ -4,7 +4,8 @@ Load zip.
 Load aux_theorems.
 Load model_evolution.
 
-Fixpoint featureFamily'Aux {model asset :Type} {H1 : Asset asset} {H2 : Model model}
+Fixpoint featureFamily'Aux {Asset model analysis :Type}
+  {H1 : @Analysis analysis Asset} {H2 : @Model model Asset}
   (rdg : RDG) (delta : RDG -> Evolution) : (string * (ADD float)) := 
   match rdg with
   | RDG_leaf s a => featureFamily (evolutionRDG rdg delta)
@@ -25,27 +26,28 @@ Fixpoint featureFamily'Aux {model asset :Type} {H1 : Asset asset} {H2 : Model mo
                        end
   end.
 
-Definition featureFamily' {model asset :Type} `{Asset asset} `{Model model}
+Definition featureFamily' {Asset model analysis :Type} `{@Analysis analysis Asset}
+  `{@Model model Asset}
   (mod : model) (delta : RDG -> Evolution) : (string * (ADD float)) := 
   featureFamily'Aux (buildRDG mod) delta.
 
-Axiom well_founded_In_rdg : forall (asset : Type) `{Asset asset},
-  well_founded (fun r1 r2 : RDG => In r1 (deps r2)).
+Axiom well_founded_In_rdg : forall (Asset : Type),
+  well_founded (fun r1 r2 : @RDG Asset => In r1 (deps r2)).
 
 (*Theorem that describe the behaviour of the partialFeatureFamilyStep in relation to featureFamily.
   Used in cases which the evolution case is different then ID*)
 
-Theorem partialFeatureFamilyStepEquivalence : forall (model asset: Type) `{Asset asset} `{Model model},
-  forall (rdg : RDG),
+Theorem partialFeatureFamilyStepEquivalence {Asset model analysis: Type}
+  `{@Analysis analysis Asset} `{@Model model Asset} : forall (rdg : RDG),
   partialFeatureFamilyStep rdg (map featureFamily (deps rdg)) = featureFamily rdg.
 Proof.
   intros. destruct rdg;
   simpl; unfold partialFeatureFamilyStep; reflexivity.
 Qed.
 
-Theorem well_founded_phi_equivalence {model asset :Type} 
-  `{Asset asset} `{Model model} : forall delta : RDG -> Evolution,
-  (forall rx : RDG, (forall ry : RDG,
+Theorem well_founded_phi_equivalence {Asset model analysis : Type} 
+  `{@Analysis analysis Asset} `{@Model model Asset} :
+  forall delta : RDG -> Evolution, (forall rx : RDG, (forall ry : RDG,
   (fun r1 r2 : RDG => In r1 (deps r2)) ry rx -> 
   (fun r : RDG => featureFamily'Aux r delta = featureFamily (evolutionRDG r delta)) ry) ->
   (fun r : RDG => featureFamily'Aux r delta = featureFamily (evolutionRDG r delta)) rx) ->
@@ -55,24 +57,25 @@ Proof.
   intros delta. apply well_founded_ind. apply well_founded_In_rdg.
 Qed.
 
-Theorem map_phi_evolution_theorem {model asset :Type} 
-  `{Asset asset} `{Model model} : forall (delta : RDG -> Evolution)
-  (l : list RDG), map featureFamily (map (fun r : RDG => evolutionRDG r delta) l) = 
+Theorem map_phi_evolution_theorem {Asset model analysis :Type} 
+  `{@Analysis analysis Asset} `{@Model model Asset} : forall
+  (delta : RDG -> Evolution) (l : list RDG), map featureFamily 
+  (map (fun r : RDG => evolutionRDG r delta) l) =
   map (fun r : RDG => featureFamily (evolutionRDG r delta)) l.
-Proof. 
+Proof.
   intros. induction l.
   - reflexivity.
   - simpl. rewrite IHl. reflexivity.
 Qed.
 
-Ltac map_deps_evolution_commutativity rdg delta D H'' asset:=
+Ltac map_deps_evolution_commutativity rdg delta D H'':=
   assert (H'' : map (fun r : RDG => featureFamily (evolutionRDG r delta)) 
   (deps rdg) = map featureFamily 
   (deps (evolutionRDG rdg delta)));
-  try(apply (commutativePhiEvolution _ asset);rewrite D;split;
+  try(apply (commutativePhiEvolution);rewrite D;split;
   intros H''';discriminate H''').
 
-Ltac map_pFeatureFamily_same_list :=
+Ltac map_pFeatureFamily_same_list H'' :=
   assert (H'' :
   forall (r : RDG) (l1 l2 : list (string * (ADD float))), l1 = l2 ->
   partialFeatureFamilyStep r l1 = partialFeatureFamilyStep r l2); 
@@ -87,21 +90,21 @@ Ltac Phi'Equivalence_list_pFeatureFamily deps0 ass s delta H :=
   (map featureFamily (deps (evolutionRDG (RDG_cons s ass deps0) delta))));
   try(intros;rewrite H;reflexivity).
 
-Ltac map_pFeatureFamily_evolution deps0 ass s delta asset:=
+Ltac map_pFeatureFamily_evolution deps0 ass s delta:=
   assert (Hsub : partialFeatureFamilyStep (RDG_cons s ass deps0) 
   (map (fun x : RDG => featureFamily'Aux x delta) deps0) = partialFeatureFamilyStep 
   (evolutionRDG (RDG_cons s ass deps0) delta) 
   (map (fun x : RDG => featureFamily'Aux x delta) deps0));
-  try(apply (subsequentModelAxiom _ asset);auto).
+  try(apply (subsequentModelAxiom );auto).
 
-Ltac simplify_case_analysis deps0 ass s delta model asset :=
+Ltac simplify_case_analysis deps0 ass s delta:=
   destruct (delta (RDG_cons s ass deps0)) eqn:D;
   simpl; rewrite D; try (apply partialFeatureFamilyStepIDEvolution in D; 
-  rewrite D;reflexivity); rewrite <- (partialFeatureFamilyStepEquivalence _ asset
+  rewrite D;reflexivity); rewrite <- (partialFeatureFamilyStepEquivalence
   (evolutionRDG (RDG_cons s ass deps0) delta)).
 
-Ltac finish_not_add_remove_case ass deps0 s delta D H' H'' asset:= 
-    map_deps_evolution_commutativity (RDG_cons s ass deps0) delta D H'' asset;
+Ltac finish_not_add_remove_case ass deps0 s delta D H' H'':= 
+    map_deps_evolution_commutativity (RDG_cons s ass deps0) delta D H'';
     rewrite <- H'' in H' at 1; auto.
 
 Ltac list_axiom := assert (H''' : 
@@ -111,34 +114,47 @@ Ltac list_axiom := assert (H''' :
 Hint Resolve In_map_theorem : core.
 Hint Resolve map_phi_evolution_theorem : core.
 
-Theorem Phi'EquivalenceAux {model asset :Type} `{Asset asset} `{Model model} :
+Theorem Phi'EquivalenceAux {Asset model analysis :Type}
+  `{@Analysis analysis Asset} `{@Model model Asset} :
   forall (rdg : RDG) (delta : RDG -> Evolution),
   featureFamily'Aux rdg delta = featureFamily (evolutionRDG rdg delta).
 Proof.
   intros. apply well_founded_phi_equivalence. intros.
   destruct rx. reflexivity.
-  Phi'Equivalence_list_pFeatureFamily deps0 ass s delta H3.
-  simplify_case_analysis deps0 ass s delta model asset;
-  try (finish_not_add_remove_case ass deps0 s delta D H' H'' asset).
+  Phi'Equivalence_list_pFeatureFamily deps0 ass s delta H2.
+  simplify_case_analysis deps0 ass s delta;
+  try (finish_not_add_remove_case ass deps0 s delta D H' H'').
   (*Add Feature Case*)
-  - map_pFeatureFamily_same_list.
+  - map_pFeatureFamily_same_list H''.
     apply depsAddEvolution in D.
     destruct D as [r [lr [H3 [H4 H5]]]]. list_axiom. 
     apply H''. rewrite H3. simpl. 
     rewrite H4. apply H'''. rewrite H5. simpl.
     rewrite map_phi_evolution_theorem. auto.
   (*Subsequent Model Evolution Case*)
-  - map_pFeatureFamily_evolution deps0 ass s delta asset.
-    map_deps_evolution_commutativity (RDG_cons s ass deps0) delta D H''' asset.
-    rewrite Hsub. auto.
+  - assert (Hsub : partialFeatureFamilyStep (RDG_cons s ass deps0) 
+    (map (fun x : RDG => featureFamily'Aux x delta) deps0) = partialFeatureFamilyStep 
+    (evolutionRDG (RDG_cons s ass deps0) delta)
+    (map (fun x : RDG => featureFamily'Aux x delta) deps0)).
+    apply subsequentModelAxiom in D.
+    unfold partialFeatureFamilyStep. unfold featureOperation.
+    destruct (evolutionRDG (RDG_cons s ass deps0) delta);
+    destruct D; simpl in H2; simpl in H3; rewrite H2; rewrite H3; auto.
+    rewrite Hsub. map_pFeatureFamily_same_list H'''. apply H'''.
+    assert (H'''' : map (fun r : RDG => featureFamily (evolutionRDG r delta)) 
+    (deps (RDG_cons s ass deps0)) =
+    map featureFamily (deps (evolutionRDG (RDG_cons s ass deps0) delta))).
+    try(apply (commutativePhiEvolution);rewrite D;split;
+    intros H'''';discriminate H''''). rewrite <- H''''.
+    apply In_map_theorem. simpl. apply H1.
   (*Remove Feature Case*)
-  - apply In_map_theorem in H2. simpl in H2. rewrite H2.
-    apply (RemoveFeatureAxiom model asset) in D. rewrite <- D.
+  - apply In_map_theorem in H1. simpl in H1. rewrite H1.
+    apply (RemoveFeatureAxiom model _ analysis) in D. rewrite <- D.
     reflexivity.
 Qed.
 
-Theorem Phi'Equivalence {model asset :Type} `{Asset asset} `{Model model} :
-  forall (m : model) (delta : RDG -> Evolution), 
+Theorem Phi'Equivalence {Asset model analysis :Type} `{@Analysis analysis Asset}
+  `{@Model model Asset} : forall (m : model) (delta : RDG -> Evolution), 
   featureFamily' m delta = featureFamily (evolutionRDG (buildRDG m) delta).
 Proof.
   intros. unfold featureFamily'. apply Phi'EquivalenceAux.
