coq_general_theory/model_evolution.v
@@ -5,20 +5,26 @@ Require Import String.
 Load ADDfloats.
 Load formula.
 
-Class Asset (asset : Type) : Type :=
-{
-  familyOperation : (string * RatExpr) -> 
-    list (string * (ADD float)) -> (string * (ADD float))
-}.
+Inductive RDG {Asset : Type} : Type :=
+| RDG_leaf (s : string) (ass : Asset)
+| RDG_cons (s : string) (ass : Asset) (deps : list RDG).
 
-Inductive RDG {asset : Type} `{Asset asset} : Type :=
-| RDG_leaf (s : string) (ass : asset)
-| RDG_cons (s : string) (ass : asset) (deps : list RDG).
-
-Definition deps {asset : Type} `{Asset asset} (rdg : RDG) : list RDG :=
+Definition deps {Asset : Type} (rdg : @RDG Asset) : list RDG :=
   match rdg with
   | RDG_leaf s a => nil
   | RDG_cons s a deps => deps
+  end.
+
+Definition asset {Asset : Type} (rdg : @RDG Asset) : Asset :=
+  match rdg with
+  | RDG_leaf s a => a
+  | RDG_cons s a deps => a
+  end.
+
+Definition rdgName {Asset : Type} (rdg : @RDG Asset) : string :=
+  match rdg with
+  | RDG_leaf s a => s
+  | RDG_cons s a deps => s
   end.
 
 Inductive Evolution : Type :=
@@ -29,16 +35,39 @@ Inductive Evolution : Type :=
   | SubsequentModelEvol
   | RemoveFeature.
 
-Class Model (model : Type) {asset : Type} `{Asset asset} : Type :=
+Fixpoint functionRecursionAux {Asset T1 T2 : Type} (f1 : (@RDG Asset) -> T1)
+  (f2 : T1 -> (list T2) -> T2) (r : @RDG Asset) : T2 :=
+  match r with
+  | RDG_leaf s ass => f2 (f1 r) nil
+  | RDG_cons s ass deps => f2 (f1 r) (map (functionRecursionAux f1 f2) deps)
+  end.
+
+Class Analysis (analysis : Type) {Asset : Type} : Type :=
+{
+  modelChecking : Asset -> RatExpr;
+  featureOperation (r : @RDG Asset) : (string * RatExpr) :=
+    match r with
+    | RDG_leaf s ass => (s , modelChecking ass)
+    | RDG_cons s ass deps => (s , modelChecking ass)
+    end;
+  familyOperation : (string * RatExpr) -> 
+    list (string * (ADD float)) -> (string * (ADD float));
+  partialFeatureFamilyStep (r : RDG)
+    (l : list (string * (ADD float))) : (string * (ADD float)) := 
+    familyOperation (featureOperation r) l;
+  featureFamily (r : RDG) : (string * (ADD float)) :=
+    functionRecursionAux featureOperation familyOperation r
+}.
+
+Class Model (model : Type) {Asset : Type} : Type :=
 {
 (*------------------------------Functions-------------------------------------------*)
 
-  buildRDG : model -> RDG;
-  featureOperation : RDG -> (string * RatExpr);
-  evolutionRDG : RDG -> (RDG -> Evolution) -> RDG;
-  AddedRDG : RDG -> (RDG -> Evolution) -> RDG;
-  ADDdepsRmvCase : RDG -> (RDG -> Evolution) -> list (string * (ADD float)) ->
-    list (string * (ADD float));
+  buildRDG : model -> (@RDG Asset);
+  evolutionRDG : (@RDG Asset) -> ((@RDG Asset) -> Evolution) -> (@RDG Asset);
+  AddedRDG : (@RDG Asset) -> ((@RDG Asset)-> Evolution) -> (@RDG Asset);
+  ADDdepsRmvCase : (@RDG Asset) -> ((@RDG Asset) -> Evolution) ->
+    list (string * (ADD float)) -> list (string * (ADD float));
 
 (*------------------------------Axioms----------------------------------------------*)
 
@@ -58,43 +87,33 @@ Class Model (model : Type) {asset : Type} `{Asset asset} : Type :=
   the evolution don't change the RDG structure*)
   commutativeDepsEvolution : forall (rdg : RDG) (delta : RDG -> Evolution) ,
   delta rdg <> AddFeature /\ delta rdg <> RemoveFeature ->
-  deps (evolutionRDG rdg delta) = map (fun r : RDG => evolutionRDG r delta) (deps rdg)
+  deps (evolutionRDG rdg delta) = map (fun r : RDG => evolutionRDG r delta) (deps rdg);
+
+  (*Axiom that describe the behaviour of a rdg evolution that the evolution case is
+  the SubsequentModelEvol case*)
+  subsequentModelAxiom : forall (r : RDG) (delta : RDG -> Evolution),
+  delta r = SubsequentModelEvol -> asset r = asset (evolutionRDG r delta) /\
+  rdgName r = rdgName (evolutionRDG r delta)
 }.
 
-Fixpoint featureFamily {asset model : Type} `{Asset asset} `{Model model}
-  (r : RDG) : (string * (ADD float)) :=
-  match r with
-  | RDG_leaf s ass => familyOperation (featureOperation r) nil
-  | RDG_cons s ass deps =>
-      familyOperation (featureOperation r) (map featureFamily deps)
-  end.
-
-Definition partialFeatureFamilyStep {asset model : Type} `{Asset asset} `{Model model}
-  (r : RDG) (l : list (string * (ADD float))) : (string * (ADD float)) := 
-  familyOperation (featureOperation r) l.
-
-(*Axiom that describe the behaviour of a rdg evolution that the evolution case is
-the SubsequentModelEvol case*)
-
-Axiom subsequentModelAxiom : forall (model asset: Type) `{Asset asset} 
-  `{Model model}, forall (r : RDG) (delta : RDG -> Evolution)
-  (l : list (string * (ADD float))), delta r = SubsequentModelEvol -> 
-  partialFeatureFamilyStep r l = partialFeatureFamilyStep (evolutionRDG r delta) l.
+Check @featureFamily.
 
 (*Axiom that describe the behaviour of a rdg evolution that the evolution case is
 the RemoveFeature case*)
 
-Axiom RemoveFeatureAxiom : forall (model asset: Type) `{Asset asset} 
-  `{Model model}, forall (r : RDG) (delta : RDG -> Evolution),
-  delta r = RemoveFeature -> 
-  ADDdepsRmvCase r delta (map (fun rdg : RDG => featureFamily (evolutionRDG rdg delta))
-  (deps r)) = map featureFamily (deps (evolutionRDG r delta)).
+Axiom RemoveFeatureAxiom : forall (model Asset analysis: Type)
+  `{@Analysis analysis Asset} `{@Model model Asset}, forall (r : RDG)
+  (delta : RDG -> Evolution), delta r = RemoveFeature -> 
+  ADDdepsRmvCase r delta (map (fun rdg : RDG => featureFamily
+  (evolutionRDG rdg delta)) (deps r)) =
+  map featureFamily (deps (evolutionRDG r delta)).
 
-Theorem commutativePhiEvolution : forall (model asset: Type) `{Asset asset} `{Model model},
+Theorem commutativePhiEvolution {Asset model analysis: Type}
+  `{@Analysis analysis Asset} `{@Model model Asset} :
   forall (rdg : RDG) (delta : RDG -> Evolution) , delta rdg <> AddFeature /\
   delta rdg <> RemoveFeature ->
-   map (fun r : RDG => featureFamily (evolutionRDG r delta)) (deps rdg) = 
-   map featureFamily (deps (evolutionRDG rdg delta)).
+  map (fun r : RDG => featureFamily (evolutionRDG r delta)) (deps rdg) = 
+  map featureFamily (deps (evolutionRDG rdg delta)).
 Proof.
   intros. assert (H' : forall (l : list RDG) (d : RDG -> Evolution),
   map (fun r : RDG => featureFamily (evolutionRDG r d)) l = map featureFamily (map 
@@ -102,6 +121,6 @@ Proof.
   { induction l.
     - intros. reflexivity.
     - intros. simpl. rewrite IHl. reflexivity. }
-  rewrite H'. apply commutativeDepsEvolution in H2.
-  rewrite H2. reflexivity.
+  rewrite H'. apply commutativeDepsEvolution in H1.
+  rewrite H1. reflexivity.
 Qed.
